polynomials over arbitrary semi-rings.

src/Verse/CryptoLib/Polynomials.v
@@ -8,48 +8,123 @@ Require Import BinNat.
 Definition term A          := (A * nat)%type.
 Definition poly (A : Type) := list (term A).
 
-(* Evaluation of polymomial at a value *)
+(**
 
-Definition evalT (eta : nat) (tm : term nat) : nat:=
-  let (coef, p) := tm in coef * eta ^ p.
+In the rather simple representation addition is just concatenation of
+the associated rings. We therefore define it for all coefficients (not
+necessarily rings).
 
-Definition eval eta (p : poly nat) : nat :=
-  let fldr (tm : term nat) sum := (sum + evalT eta tm)
-  in List.fold_right fldr 0 p.
-
-
+ *)
 Definition add {A : Type}(p1 p2 : poly A) := p1 ++ p2.
 
-Definition mulTT (t1 t2 : term nat) : term nat :=
-  let (coef1, p1) := t1 in
-  let (coef2, p2) := t2 in
-  (coef1 * coef2 , p1 + p2).
+(** Type classes for ring *)
 
-Definition mulTP (t : term nat) : poly nat -> poly nat :=
-  List.map (mulTT t).
+Class Semi_Ring_Zero S := semi_ring_zero : S.
+Class Semi_Ring_One  S := semi_ring_one : S.
+Class Semi_Ring_Add  S := semi_ring_add : S -> S -> S.
+Class Semi_Ring_Mul  S := semi_ring_mul : S -> S -> S.
 
-Fixpoint mul (p1 p2 : poly nat) : poly nat :=
-  match p1 with
-  | [] => []
-  | (t :: ts) => add (mulTP t p2)  (mul ts p2)
+(*
+
+This is needed for proving correctness for arbitrary rings
+
+*)
+Class Semi_Ring_Eq   S := semi_ring_eq : S -> S -> Prop.
+
+Class Semi_Ring S
+      `{Semi_Ring_Zero S}
+      `{Semi_Ring_One S}
+      `{Semi_Ring_Add S}
+      `{Semi_Ring_Mul S}
+      `{Semi_Ring_Eq S}
+  := {}. (* semi_ring_spec: semi_ring_theory semi_ring_zero
+                                      semi_ring_one
+                                      semi_ring_add
+                                      semi_ring_mul
+                                      semi_ring_eq. *)
+
+
+Declare Scope ring_scope.
+Delimit Scope ring_scope with ring.
+Notation "0" := semi_ring_zero : ring_scope.
+Notation "1" := semi_ring_one : ring_scope.
+Infix "+" := semi_ring_add   : ring_scope.
+Infix "*" := semi_ring_mul   : ring_scope.
+
+Fixpoint pow {SR : Type}`{Semi_Ring SR}(eta : SR)(n : nat) :=
+  match n with
+  | 0   => 1%ring
+  | S m => (eta  * (pow eta m))%ring
   end.
 
+Infix "^" := pow :ring_scope.
+
+
+Section Operations.
+
+  Context {SR : Type}`{Semi_Ring SR}.
+
+  (* Evaluation of polymomial at a value *)
+
+  Definition evalT (eta : SR) (tm : term SR) : SR :=
+    let (coef, p) := tm in (coef * eta ^ p)%ring.
+
+  Definition eval eta (p : poly SR) : SR :=
+    let fldr (tm : term SR) sum := (sum + evalT eta tm)%ring
+    in List.fold_right fldr 0%ring p.
+
+
+  Definition mulTT (t1 t2 : term SR) : term SR :=
+    let (coef1, p1) := t1 in
+    let (coef2, p2) := t2 in
+    ((coef1 * coef2)%ring , p1 + p2).
+
+  Definition mulTP (t : term SR) : poly SR -> poly SR :=
+    List.map (mulTT t).
+
+  Fixpoint mul (p1 p2 : poly SR) : poly SR :=
+    match p1 with
+    | [] => []
+    | (t :: ts) => add (mulTP t p2)  (mul ts p2)
+    end.
+
+End Operations.
+
+Instance nat_zero : Semi_Ring_Zero nat := 0.
+Instance nat_one : Semi_Ring_One nat := 1.
+Instance nat_add : Semi_Ring_Add nat := Nat.add.
+Instance nat_mul : Semi_Ring_Mul nat := Nat.mul.
+Instance nat_eq  : Semi_Ring_Eq nat  := eq.
+Instance nat_semi_ring : Semi_Ring nat  := {}.
 
 Section Spec.
   Context {eta : nat}.
 
+  Ltac specialise_to_nat :=
+    repeat (unfold semi_ring_add; unfold semi_ring_mul; unfold nat_add; unfold nat_mul).
 
-  Lemma add_spec : forall p1 p2, eval eta p1 + eval eta p2 = eval eta (add p1 p2).
-  Proof.
+  Ltac specialise_nat_ring:=
+     specialise_to_nat; ring.
+
+  Lemma add_spec : forall (p1 p2 : poly nat), eval eta p1 + eval eta p2 = eval eta (add p1 p2).
     intros.
     induction p1; simpl; trivial.
     rewrite <- IHp1.
-    ring.
+    specialise_nat_ring.
+  Qed.
+
+  Lemma power_lemma : forall (x : nat)(p : nat), pow x p = x ^ p.
+  Proof using Type.
+    intros.
+    induction p; simpl; trivial.
+    rewrite <- IHp. easy.
   Qed.
 
   Lemma mulTT_spec : forall t1 t2, evalT eta (mulTT t1 t2) = evalT eta t1 * evalT eta t2.
     intros; destruct t1; destruct t2; simpl.
-    rewrite Nat.pow_add_r; ring.
+    repeat rewrite power_lemma.
+    rewrite Nat.pow_add_r.
+    specialise_nat_ring.
   Qed.
 
   Lemma mulTP_spec : forall tm p, eval eta (mulTP tm p) = evalT eta tm * eval eta p.
@@ -57,16 +132,15 @@ Section Spec.
     induction p; simpl; trivial.
     rewrite IHp.
     rewrite (mulTT_spec).
-    ring.
+    specialise_nat_ring.
   Qed.
 
   Lemma mul_spec : forall p1 p2, eval eta (mul p1 p2) = eval eta p1 * eval eta p2.
     intros.
     induction p1; simpl; trivial.
-    ring_simplify.
-    rewrite <- IHp1.
-    rewrite <- mulTP_spec.
     rewrite <- add_spec.
-    ring.
+    rewrite mulTP_spec.
+    rewrite IHp1.
+    specialise_nat_ring.
   Qed.
 End Spec.
